\documentclass{article}
\usepackage{amsmath}
\usepackage{amsthm}
\usepackage{amsfonts}
\usepackage{bm}
\usepackage[usenames,dvipsnames]{xcolor}
\usepackage{tikz}
\usepackage{hyperref}

\hypersetup{
    colorlinks,
    linkcolor={red!30!black},
    citecolor={blue!50!black},
    urlcolor={blue!80!black}
}


\begin{document}

\title{PDE lectures}
\author{ \vspace{-10ex} }
\date{ \vspace{-10ex} }
\maketitle

\tableofcontents

\section{Solve PDE via change of variables}

How to solve PDE via change of variables, \url{https://www.youtube.com/watch?v=VIqKKq_jZu0}.

Example of how to solve PDE via change of variables, \url{https://www.youtube.com/watch?v=HouEinUtASE}

\subsection{Method}

General case
$$
a \, u_x + b \, u_y = f,
$$
We want to simplify the PDE via change of variables.
$$
\xi = \xi(x, y), \eta = \eta(x, y).
$$

Using the chain rule, we get
$$
(a \xi_x + b \xi_y) u_\xi + (a \eta_x + b \eta_y) u_\eta = f.
$$
Now if $a \xi_x + b \xi_y$ is zero,
the equation is simplified with only one partial derivative $u_\eta$.
Further, if $\eta(x, y) = x$, then it is simply $a u_\eta = f$.
So we want to solve
$$
\begin{aligned}
a \xi_x + b \xi_y = 0, \\
a u_\eta = f.
\end{aligned}
$$

Now the first equation can be solved along the curve
$$
\frac{ dx } { a } = \frac { dy } { b }.
$$
which will yield a curve $\phi(x, y) = C$.
%
We will then choose $\xi = \phi(x, y)$.


\subsection{Example}

Solve (for $x > 0$)
$$
x \, u_x - y \, u_y + u  = 2.
$$

The goal is to simplify the PDE using new variables $(\xi, \eta)$.

$$
dy/dx = b/a = - y/x.
$$
Integrating this we get $xy = C$.
So we choose $\xi(x, y) = C = xy$.

The other choice is $\eta(x, y) = x$.

Consider $u(\xi, \eta)$,
$$
u_x = u_\xi \xi_x + u_\eta \eta_x = u_\xi \, y + u_\eta,
\quad
u_y = u_\xi \xi_y + u_\eta \eta_y = u_\xi \, x.
$$
So
$$
x \, y \, (u_\xi \, y + u_\eta)
- y \, u_\xi \, x + u = 2,
$$
We get
$$
\eta \, u_\eta + u = 2.
$$
This is equivalent to $\partial ( \eta \, u_\eta ) /\partial \eta = 2$.
So the solution is
$\eta \, u = 2 \, \eta + K(\xi)$.
In terms of $x$ and $y$, we get
$$
u = 2 + K(xy)/x.
$$



\end{document}
